% Font size, paper type
\documentclass[12pt]{article}
% Aesthetic margins
\usepackage[margin=1in]{geometry}
% Core math packages,
% Mathtools loads amsmath, and amsmath gives basic math symbs
% Amsfonts & amssymb are misc. symbols you might need
\usepackage{mathtools, amsfonts, amssymb}
% Links in a pdf
\usepackage{hyperref}
% Use in pictures, graphs, and figures
\usepackage{graphicx}
% Header package
\usepackage{fancyhdr}
% Underlining with line breaks
\usepackage{ulem}
% Adjust accordingly given warning messages
\setlength{\headheight}{15pt}

% Sets footer
\pagestyle{fancy}
% Removes default footer style
\fancyhf{}

\rhead{
  Shengdong Li
  Calc 3
}

\rfoot{
  Page \thepage
}

% Makes links look more appealling
\hypersetup{
    colorlinks=true,
    linkcolor=blue,
    filecolor=magenta,      
    urlcolor=cyan,
}

% \usepackage{indentfirst}

\begin{document}
\title{Initial Post}
\author{by Shengdong Li}
\date{19 November 2020}
\maketitle

% Remember to use \ldots
\section{\texorpdfstring{$\frac{1}{1-x}$}{Lg}}
To find the maclaurin series for $\frac{1}{1-x}$, first find the first 5 derivatives of $f(x)$
\begin{align}
  f\left(x\right)                  & =\left(1-x\right)^{-1}                                                                \\
  f'\left(x\right)                 & =\left(1-x\right)^{-2}                                                                \\
  f''\left(x\right)                & =2\left(1-x\right)^{-3}                                                               \\
  f'''\left(x\right)               & =6\left(1-x\right)^{-4}                                                               \\
  f^{\left(4\right)}\left(x\right) & =24\left(1-x\right)^{-5}                                                              \\
  f^{\left(5\right)}\left(x\right) & =120\left(1-x\right)^{-6}                                                             \\
  \intertext{Now we know that in a maclaurin series the function is centered at $a=0$. We plugin $0$ into our previously calculated derivatives}
  f\left(0\right)                  & =1                                                                                    \\
  f'\left(0\right)                 & =1                                                                                    \\
  f''\left(0\right)                & =2\cdot1                                                                              \\
  f'''\left(0\right)               & =6\cdot1                                                                              \\
  f^{\left(4\right)}\left(0\right) & =24\cdot1                                                                             \\
  f^{\left(5\right)}\left(0\right) & =120\cdot1                                                                            
\end{align}
We can plug these derivatives into the general formula for taylor polynomials
\begin{align}
  \Aboxed{\frac{1}{1-x}                    & =1+x+\frac{2x^{2}}{2!}+\frac{6x^{3}}{3!}+\frac{24x^{4}}{4!}+\frac{120x^{5}}{5!}+...}
\end{align}
The final taylor series would then be
\begin{align}
  \frac{1}{1-x}                    & = \sum_{n=0}^{\infty}\frac{n!x^{n}}{n!}=\sum_{n=0}^{\infty}x^{n}                      \\
\end{align}
Another way to approach finding the series is to define $f^{(n)}(x)$. From the derivatives above, we can see that the $n$th derivative $f^{(n)}(x)$ would be $n!$
\begin{align}
  f^{\left(n\right)}\left(x\right) & =n!                                                                                   \\
  \frac{1}{1-x}                    & = \sum_{n=0}^{\infty}\frac{f^{\left(n\right)}\left(x\right)\cdot\left(x-a\right)}{n!} \\
  \frac{1}{1-x}                    & = \sum_{n=0}^{\infty}\frac{n!\cdot x}{n!}                                             \\
\end{align}
Plugging into the formula, the $n!$s cancel, leaving
\begin{align}
\Aboxed{\frac{1}{1-x}                    & = \sum_{n=0}^{\infty}x}
\end{align}
\section{\texorpdfstring{$\left(1-2x\right)^{-1}$}{Lg}}
To find the maclaurin series for $\left(1-2x\right)^{-1}$, find the first 5 derivatives of $f(x)$ again
\begin{align}
  f\left(x\right)                  & =\left(1-2x\right)^{-1}                                                                 \\
  f'\left(x\right)                 & =2\left(1-2x\right)^{-2}                                                                \\
  f''\left(x\right)                & =8\left(1-2x\right)^{-3}                                                                \\
  f'''\left(x\right)               & =48\left(1-2x\right)^{-4}                                                               \\
  f^{\left(4\right)}\left(x\right) & =384\left(1-2x\right)^{-5}                                                              \\
  f^{\left(5\right)}\left(x\right) & =3840\left(1-2x\right)^{-6}                                                             \\
  \intertext{Plugin $x=0$ for maclaurin series}
  f\left(0\right)                  & =1                                                                                      \\
  f'\left(0\right)                 & =2                                                                                      \\
  f''\left(0\right)                & =8                                                                                      \\
  f'''\left(0\right)               & =48                                                                                     \\
  f^{\left(4\right)}\left(0\right) & =384                                                                                    \\
  f^{\left(5\right)}\left(0\right) & =3840                                                                                   
\end{align}
\begin{align}
  \intertext{Then plug in the results into the taylor formula to get the first 5 terms}
  \frac{1}{1-x}                    & =1+2x+\frac{8x^{2}}{2!}+\frac{48x^{3}}{3!}+\frac{384x^{4}}{4!}+\frac{3840x^{5}}{5!}+... \\
                                   \Aboxed{& =1+2x+4x^{2}+8x^{3}+16x^{4}+32x^{5}+...}                                                 \\
                                   & = \sum_{n=0}^{\infty}2^{n}x^{n}                                                         \\
                                   \Aboxed{& = \sum_{n=0}^{\infty}\left(2x\right)^{n}}                                                
\end{align}
\begin{align}
  \intertext{Another way we could approach this problem is to find $f^{(n)}(x)$ and plug that directly into the formula}
  \frac{1}{1-x}                    & =\frac{f^{\left(n\right)}\left(x\right)\cdot\left(x-a\right)}{n!}                       \\
  f^{\left(n\right)}\left(x\right) & =n!\cdot2^{n}                                                                           \\
                                   & =\frac{n!\cdot2^{n}\cdot x}{n!}                                                         \\
                                   & =2^{n}x^{n}                                                                             \\
                                   & =\sum_{n=0}^{\infty}\left(2x\right)^{n}                                                                    \\
\end{align}
\section{\texorpdfstring{$\frac{1}{1-x^{2}}$}{Lg}}
To find the maclaurin series for $\frac{1}{1-x^{2}}$, find the first 5 derivatives of $f(x)$
\begin{align}
  f\left(x\right)                  & =\frac{1}{1-x^{2}}                                                  \\
  f\left(x\right)                  & =\left(1-x^{2}\right)^{-1}                                          \\
  f'\left(x\right)                 & =2x\left(1-x^{2}\right)^{-2}                                        \\
  f''\left(x\right)                & =\frac{2\left(1+3x^{2}\right)}{\left(1-x^{2}\right)^{3}}            \\
  f'''\left(x\right)               & =24x\left(\frac{1+x^{2}}{\left(1-x^{2}\right)^{4}}\right)           \\
  f^{\left(4\right)}\left(x\right) & =24\left(\frac{5x^{4}+10x^{2}+1}{\left(1-x^{2}\right)^{5}}\right)   \\
  f^{\left(5\right)}\left(x\right) & =240x\left(\frac{3x^{4}+10x^{2}+3}{\left(1-x^{2}\right)^{6}}\right) \\
  \intertext{Next, plugin $x=0$ for a maclaurin series}
  f\left(0\right)                  & =1                                                                  \\
  f'\left(0\right)                 & =0                                                                  \\
  f''\left(0\right)                & =2                                                                  \\
  f'''\left(0\right)               & =0                                                                  \\
  f^{\left(4\right)}\left(0\right) & =24                                                                 \\
  f^{\left(5\right)}\left(0\right) & =0                                                                  \\
  \intertext{Plugging the results into the taylor formula gives}
  \Aboxed{\frac{1}{1-x^{2}}                & =1+\frac{2x^{2}}{2!}+\frac{24x^{4}}{4!}+...}                         \\
  \Aboxed{\frac{1}{1-x^{2}}                & =\sum_{n=0}^{\infty}x^{2n}}                                         
\end{align}

\end{document}